ocaml/src/PrettyQuery.mli
@@ -39,8 +39,8 @@ val pretty_nnrc_core : QcertCompiler.nnrc_core pretty_fun
 val pretty_nnrc : QcertCompiler.nnrc pretty_fun
 val pretty_nnrcmr : QcertCompiler.nnrcmr pretty_fun
 val pretty_cldmr : QcertCompiler.cldmr pretty_fun
-val pretty_dnnrc_dataframe : QcertCompiler.dnnrc_dataframe pretty_fun
-val pretty_dnnrc_dataframe_typed : QcertCompiler.dnnrc_typed pretty_fun
+val pretty_dnnrc : QcertCompiler.dnnrc pretty_fun
+val pretty_dnnrc_typed : QcertCompiler.dnnrc_typed pretty_fun
 val pretty_javascript : QcertCompiler.javascript pretty_fun
 val pretty_java : QcertCompiler.java pretty_fun
 val pretty_spark_rdd : QcertCompiler.spark_rdd pretty_fun
