coq/DNNRC/Lang/DNNRC.v
@@ -23,13 +23,13 @@ Section DNNRC.
   Context {fruntime:foreign_runtime}.
   Context {ftype: ForeignType.foreign_type}.
 
-  Definition dnnrc_dataframe := @dnnrc _ unit dataframe.
+  Definition dnnrc := @dnnrc_base _ unit dataframe.
 
   Section Top.
     Context (h:brand_relation_t).
 
-    Definition dnnrc_dataframe_eval_top (q:dnnrc_dataframe) (cenv:dbindings) : option data :=
-      lift unlocalize_data (dnnrc_eval h (rec_sort cenv) nil q).
+    Definition dnnrc_eval_top (q:dnnrc) (cenv:dbindings) : option data :=
+      lift unlocalize_data (dnnrc_base_eval h (rec_sort cenv) nil q).
 
   End Top.
 
