coq/DNNRC/Lang/DNNRCBaseEq.v
@@ -37,99 +37,99 @@ Section DNNRCBaseEq.
   (** Equivalence between expressions in the 
       Distributed Nested Relational Calculus *)
 
-  Definition dnnrc_eq (e1 e2:@dnnrc _ A plug_type) : Prop :=
+  Definition dnnrc_base_eq (e1 e2:@dnnrc_base _ A plug_type) : Prop :=
     forall (h:brand_relation_t) (dcenv denv:dbindings),
       Forall (ddata_normalized h) (map snd dcenv) ->
       Forall (ddata_normalized h) (map snd denv) ->
-      dnnrc_eval h dcenv denv e1 = dnnrc_eval h dcenv denv e2.
+      dnnrc_base_eval h dcenv denv e1 = dnnrc_base_eval h dcenv denv e2.
 
-  Global Instance dnnrc_equiv : Equivalence dnnrc_eq.
+  Global Instance dnnrc_base_equiv : Equivalence dnnrc_base_eq.
   Proof.
     constructor.
-    - unfold Reflexive, dnnrc_eq.
+    - unfold Reflexive, dnnrc_base_eq.
       intros; reflexivity.
-    - unfold Symmetric, dnnrc_eq.
+    - unfold Symmetric, dnnrc_base_eq.
       intros; rewrite (H _ dcenv denv) by trivial; reflexivity.
-    - unfold Transitive, dnnrc_eq.
+    - unfold Transitive, dnnrc_base_eq.
       intros; rewrite (H _ dcenv denv) by trivial;
       rewrite (H0 _ dcenv denv) by trivial; reflexivity.
   Qed.
 
-  (* all the dnnrc constructors are proper wrt. equivalence *)
+  (* all the dnnrc_base constructors are proper wrt. equivalence *)
 
   (* DNNRCGetConstant *)
-  Global Instance dgetconstant_proper : Proper (eq ==> eq ==> dnnrc_eq) DNNRCGetConstant.
+  Global Instance dgetconstant_proper : Proper (eq ==> eq ==> dnnrc_base_eq) DNNRCGetConstant.
   Proof.
-    unfold Proper, respectful, dnnrc_eq.
+    unfold Proper, respectful, dnnrc_base_eq.
     intros; subst; reflexivity.
   Qed.
 
   (* DNNRCVar *)
-  Global Instance dvar_proper : Proper (eq ==> eq ==> dnnrc_eq) DNNRCVar.
+  Global Instance dvar_proper : Proper (eq ==> eq ==> dnnrc_base_eq) DNNRCVar.
   Proof.
-    unfold Proper, respectful, dnnrc_eq.
+    unfold Proper, respectful, dnnrc_base_eq.
     intros; subst; reflexivity.
   Qed.
 
   (* DNNRCConst *)
   
-  Global Instance dconst_proper : Proper (eq ==> eq ==> dnnrc_eq) DNNRCConst.
+  Global Instance dconst_proper : Proper (eq ==> eq ==> dnnrc_base_eq) DNNRCConst.
   Proof.
-    unfold Proper, respectful, dnnrc_eq.
+    unfold Proper, respectful, dnnrc_base_eq.
     intros; subst; reflexivity.
   Qed.
 
   (* DNNRCBinop *)
   
-  Global Instance dbinop_proper : Proper (eq ==> binop_eq ==> dnnrc_eq ==> dnnrc_eq ==> dnnrc_eq) DNNRCBinop.
+  Global Instance dbinop_proper : Proper (eq ==> binop_eq ==> dnnrc_base_eq ==> dnnrc_base_eq ==> dnnrc_base_eq) DNNRCBinop.
   Proof.
-    unfold Proper, respectful, dnnrc_eq.
+    unfold Proper, respectful, dnnrc_base_eq.
     intros; simpl. subst.
     rewrite H1 by trivial.
     rewrite H2 by trivial.
-    case_eq (dnnrc_eval h dcenv denv y1);
-      case_eq (dnnrc_eval h dcenv denv y2); intros; simpl; trivial.
+    case_eq (dnnrc_base_eval h dcenv denv y1);
+      case_eq (dnnrc_base_eval h dcenv denv y2); intros; simpl; trivial.
     destruct d0; destruct d; try reflexivity; simpl.
     rewrite H0; [reflexivity| | ].
-    apply (dnnrc_eval_normalized_local h dcenv denv y1); try assumption.
-    apply (dnnrc_eval_normalized_local h dcenv denv y1); try assumption.
+    apply (dnnrc_base_eval_normalized_local h dcenv denv y1); try assumption.
+    apply (dnnrc_base_eval_normalized_local h dcenv denv y1); try assumption.
   Qed.
 
   (* DNNRCUnnop *)
   
-  Global Instance dunop_proper : Proper (eq ==> unaryop_eq ==> dnnrc_eq ==> dnnrc_eq) DNNRCUnop.
+  Global Instance dunop_proper : Proper (eq ==> unaryop_eq ==> dnnrc_base_eq ==> dnnrc_base_eq) DNNRCUnop.
   Proof.
-    unfold Proper, respectful, dnnrc_eq.
+    unfold Proper, respectful, dnnrc_base_eq.
     intros; simpl. subst.
     rewrite H1 by trivial.
-    case_eq (dnnrc_eval h dcenv denv y1); simpl; trivial; intros.
+    case_eq (dnnrc_base_eval h dcenv denv y1); simpl; trivial; intros.
     destruct d; try reflexivity; simpl.
     rewrite H0; [reflexivity| ].
-    apply (dnnrc_eval_normalized_local h dcenv denv y1); try assumption.
+    apply (dnnrc_base_eval_normalized_local h dcenv denv y1); try assumption.
   Qed.
     
   (* DNNRCLet *)
   
-  Global Instance dlet_proper : Proper (eq ==> eq ==> dnnrc_eq ==> dnnrc_eq ==> dnnrc_eq) DNNRCLet.
+  Global Instance dlet_proper : Proper (eq ==> eq ==> dnnrc_base_eq ==> dnnrc_base_eq ==> dnnrc_base_eq) DNNRCLet.
   Proof.
-    unfold Proper, respectful, dnnrc_eq.
+    unfold Proper, respectful, dnnrc_base_eq.
     intros; simpl. rewrite H0; clear H0; rewrite H1 by trivial; clear H1.
-    case_eq (dnnrc_eval h dcenv denv y1); simpl; trivial; intros.
+    case_eq (dnnrc_base_eval h dcenv denv y1); simpl; trivial; intros.
     rewrite H2; eauto.
     constructor; eauto.
     simpl.
-    eapply (dnnrc_eval_normalized h dcenv denv y1); eauto.
+    eapply (dnnrc_base_eval_normalized h dcenv denv y1); eauto.
   Qed.
 
   (* DNNRCFor *)
 
   Hint Resolve data_normalized_dcoll_in.
 
-  Global Instance dfor_proper : Proper (eq ==> eq ==> dnnrc_eq ==> dnnrc_eq ==> dnnrc_eq) DNNRCFor.
+  Global Instance dfor_proper : Proper (eq ==> eq ==> dnnrc_base_eq ==> dnnrc_base_eq ==> dnnrc_base_eq) DNNRCFor.
   Proof.
-    unfold Proper, respectful, dnnrc_eq.
+    unfold Proper, respectful, dnnrc_base_eq.
     intros; simpl. rewrite H1 by trivial; clear H1. subst.
-    case_eq (dnnrc_eval h dcenv denv y1); simpl; trivial; intros.
+    case_eq (dnnrc_base_eval h dcenv denv y1); simpl; trivial; intros.
     destruct d; try reflexivity; simpl.
     { destruct d; try reflexivity; simpl.
       f_equal.
@@ -137,7 +137,7 @@ Section DNNRCBaseEq.
       rewrite H2; simpl; eauto.
       constructor; [|assumption].
       assert (ddata_normalized h (Dlocal (dcoll l))).
-      - eapply (dnnrc_eval_normalized _ dcenv denv); eauto.
+      - eapply (dnnrc_base_eval_normalized _ dcenv denv); eauto.
       - inversion H1; subst; clear H1.
         econstructor.
         inversion H6; subst; clear H6.
@@ -148,7 +148,7 @@ Section DNNRCBaseEq.
       rewrite H2; simpl; eauto.
       constructor; [|assumption].
       assert (ddata_normalized h (Ddistr l)).
-      - eapply (dnnrc_eval_normalized _ dcenv denv); eauto.
+      - eapply (dnnrc_base_eval_normalized _ dcenv denv); eauto.
       - inversion H1; subst; clear H1.
         constructor.
         rewrite Forall_forall in H6.
@@ -157,20 +157,20 @@ Section DNNRCBaseEq.
 
   (* DNNRCIf *)
   
-  Global Instance dif_proper : Proper (eq ==> dnnrc_eq ==> dnnrc_eq ==> dnnrc_eq ==> dnnrc_eq) DNNRCIf.
+  Global Instance dif_proper : Proper (eq ==> dnnrc_base_eq ==> dnnrc_base_eq ==> dnnrc_base_eq ==> dnnrc_base_eq) DNNRCIf.
   Proof.
-    unfold Proper, respectful, dnnrc_eq.
+    unfold Proper, respectful, dnnrc_base_eq.
     intros; simpl. subst. rewrite H0 by trivial; clear H0.
-    case_eq (dnnrc_eval h dcenv denv y0); simpl; trivial; intros.
+    case_eq (dnnrc_base_eval h dcenv denv y0); simpl; trivial; intros.
     destruct d; try reflexivity; simpl.
     destruct d; try reflexivity; simpl.
     destruct b; eauto.
   Qed.
 
   (* DNNRCEither *)
-  Global Instance deither_proper : Proper (eq ==> dnnrc_eq ==> eq ==> dnnrc_eq ==> eq ==> dnnrc_eq ==> dnnrc_eq) DNNRCEither.
+  Global Instance deither_proper : Proper (eq ==> dnnrc_base_eq ==> eq ==> dnnrc_base_eq ==> eq ==> dnnrc_base_eq ==> dnnrc_base_eq) DNNRCEither.
   Proof.
-    unfold Proper, respectful, dnnrc_eq.
+    unfold Proper, respectful, dnnrc_base_eq.
     intros; simpl. subst.
     rewrite H0 by trivial.
     match_case; intros ? eqq1. match_destr.
@@ -178,10 +178,10 @@ Section DNNRCBaseEq.
       rewrite Forall_forall; intros.
       inversion H; subst.
       unfold olift, checkLocal in eqq1.
-      case_eq (dnnrc_eval h dcenv denv y0); intros; rewrite H1 in eqq1; try congruence;
+      case_eq (dnnrc_base_eval h dcenv denv y0); intros; rewrite H1 in eqq1; try congruence;
       destruct d0; try congruence; inversion eqq1; subst.
       assert (ddata_normalized h (Dlocal (dleft d))).
-      apply (@dnnrc_eval_normalized _ _ _ h dcenv _ denv y0); assumption.
+      apply (@dnnrc_base_eval_normalized _ _ _ h dcenv _ denv y0); assumption.
       inversion H3; subst; clear H3.
       inversion H8; subst; clear H8.
       constructor; assumption.
@@ -190,55 +190,55 @@ Section DNNRCBaseEq.
       rewrite Forall_forall; intros.
       inversion H; subst.
       unfold olift, checkLocal in eqq1.
-      case_eq (dnnrc_eval h dcenv denv y0); intros; rewrite H1 in eqq1; try congruence;
+      case_eq (dnnrc_base_eval h dcenv denv y0); intros; rewrite H1 in eqq1; try congruence;
       destruct d0; try congruence; inversion eqq1; subst.
       assert (ddata_normalized h (Dlocal (dright d))).
-      apply (@dnnrc_eval_normalized _ _ _ h dcenv plug denv y0); assumption.
+      apply (@dnnrc_base_eval_normalized _ _ _ h dcenv plug denv y0); assumption.
       inversion H3; subst; clear H3.
       inversion H8; subst; clear H8.
       constructor; assumption.
       rewrite Forall_forall in H6. auto.
   Qed.
 
-    (* DNNRCGroupBy *)
-  Global Instance dgroupby_proper : Proper (eq ==> eq ==> eq ==> dnnrc_eq ==>dnnrc_eq) DNNRCGroupBy.
+  (* DNNRCGroupBy *)
+  Global Instance dgroupby_proper : Proper (eq ==> eq ==> eq ==> dnnrc_base_eq ==>dnnrc_base_eq) DNNRCGroupBy.
   Proof.
-    unfold Proper, respectful, dnnrc_eq.
+    unfold Proper, respectful, dnnrc_base_eq.
     intros; simpl; subst.
     trivial.
   Qed.
 
   (* DNNRCCollect *)
-  Global Instance dcollect_proper : Proper (eq ==> dnnrc_eq ==> dnnrc_eq) DNNRCCollect.
+  Global Instance dcollect_proper : Proper (eq ==> dnnrc_base_eq ==> dnnrc_base_eq) DNNRCCollect.
   Proof.
-    unfold Proper, respectful, dnnrc_eq.
+    unfold Proper, respectful, dnnrc_base_eq.
     intros; simpl. subst.
     rewrite H0 by trivial.
     reflexivity.
   Qed.
     
   (* DNNRCDispatch *)
-  Global Instance ddispatch_proper : Proper (eq ==> dnnrc_eq ==> dnnrc_eq) DNNRCDispatch.
+  Global Instance ddispatch_proper : Proper (eq ==> dnnrc_base_eq ==> dnnrc_base_eq) DNNRCDispatch.
   Proof.
-    unfold Proper, respectful, dnnrc_eq.
+    unfold Proper, respectful, dnnrc_base_eq.
     intros; simpl. subst.
     rewrite H0 by trivial.
     reflexivity.
   Qed.
 
-  Global Instance dalg_proper : Proper (eq ==> eq ==> Forall2 (fun n1 n2  => fst n1 = fst n2 /\ dnnrc_eq (snd n1) (snd n2)) ==> dnnrc_eq) DNNRCAlg.
+  Global Instance dalg_proper : Proper (eq ==> eq ==> Forall2 (fun n1 n2  => fst n1 = fst n2 /\ dnnrc_base_eq (snd n1) (snd n2)) ==> dnnrc_base_eq) DNNRCAlg.
   Proof.
-    unfold Proper, respectful, dnnrc_eq.
+    unfold Proper, respectful, dnnrc_base_eq.
     intros; simpl; subst.
     cut ((map
-         (fun x : string * @dnnrc _ A plug_type =>
-          match dnnrc_eval h dcenv denv (snd x) with
+         (fun x : string * @dnnrc_base _ A plug_type =>
+          match dnnrc_base_eval h dcenv denv (snd x) with
           | Some (Dlocal _) => None
           | Some (Ddistr coll) => Some (fst x, coll)
           | None => None
           end) x1) = (map
-         (fun x : string * @dnnrc _ A plug_type =>
-          match dnnrc_eval h dcenv denv (snd x) with
+         (fun x : string * @dnnrc_base _ A plug_type =>
+          match dnnrc_base_eval h dcenv denv (snd x) with
           | Some (Dlocal _) => None
           | Some (Ddistr coll) => Some (fst x, coll)
           | None => None
@@ -252,7 +252,7 @@ Section DNNRCBaseEq.
 
 End DNNRCBaseEq.
 
-Notation "X ≡ᵈ Y" := (dnnrc_eq X Y) (at level 90) : dnnrc_scope.                             (* ≡ = \equiv *)
+Notation "X ≡ᵈ Y" := (dnnrc_base_eq X Y) (at level 90) : dnnrc_scope.                             (* ≡ = \equiv *)
 
 (* 
 *** Local Variables: ***
