coq/DNNRC/Typing/TDNNRCBase.v
@@ -58,77 +58,77 @@ Section TDNNRCBase.
         end
       end.
 
-    Inductive dnnrc_type `{tplug: TAlgPlug} {A} : tdbindings -> @dnnrc _ A plug_type -> drtype -> Prop :=
+    Inductive dnnrc_base_type `{tplug: TAlgPlug} {A} : tdbindings -> @dnnrc_base _ A plug_type -> drtype -> Prop :=
     | TDNNRCGetConstant {τout} tenv s :
         forall (a:A),
           tdot τconstants s = Some τout ->
-          dnnrc_type tenv (DNNRCGetConstant a s) τout
+          dnnrc_base_type tenv (DNNRCGetConstant a s) τout
     | TDNNRCVar {τout} tenv v :
         forall (a:A),
           lookup equiv_dec tenv v = Some τout ->
-          dnnrc_type tenv (DNNRCVar a v) τout
+          dnnrc_base_type tenv (DNNRCVar a v) τout
     | TDNNRCConst {τout} tenv c :
         forall (a:A),
           data_type (normalize_data brand_relation_brands c) τout ->
-          dnnrc_type tenv (DNNRCConst a c) (Tlocal τout)
+          dnnrc_base_type tenv (DNNRCConst a c) (Tlocal τout)
     | TDNNRCBinop  {τ₁ τ₂ τout} tenv b e1 e2 :
         forall (a:A),
           binOp_type b τ₁ τ₂ τout ->
-          dnnrc_type tenv e1 (Tlocal τ₁) ->
-          dnnrc_type tenv e2 (Tlocal τ₂) ->
-          dnnrc_type tenv (DNNRCBinop a b e1 e2) (Tlocal τout)
+          dnnrc_base_type tenv e1 (Tlocal τ₁) ->
+          dnnrc_base_type tenv e2 (Tlocal τ₂) ->
+          dnnrc_base_type tenv (DNNRCBinop a b e1 e2) (Tlocal τout)
     | TDNNRCUnop {τ₁ τout} tenv u e1 :
         forall (a:A), 
           unaryOp_type u τ₁ τout ->
-          dnnrc_type tenv e1 (Tlocal τ₁) ->
-          dnnrc_type tenv (DNNRCUnop a u e1) (Tlocal τout)
+          dnnrc_base_type tenv e1 (Tlocal τ₁) ->
+          dnnrc_base_type tenv (DNNRCUnop a u e1) (Tlocal τout)
     | TDNNRCLet {τ₁ τ₂} v tenv e1 e2 :
         forall (a:A), 
-          dnnrc_type tenv e1 τ₁ ->
-          dnnrc_type ((v,τ₁)::tenv) e2 τ₂ ->
-          dnnrc_type tenv (DNNRCLet a v e1 e2) τ₂
+          dnnrc_base_type tenv e1 τ₁ ->
+          dnnrc_base_type ((v,τ₁)::tenv) e2 τ₂ ->
+          dnnrc_base_type tenv (DNNRCLet a v e1 e2) τ₂
     | TDNNRCForLocal {τ₁ τ₂} v tenv e1 e2 :
         forall (a:A),
-          dnnrc_type tenv e1 (Tlocal (Coll τ₁)) ->
-          dnnrc_type ((v,(Tlocal τ₁))::tenv) e2 (Tlocal τ₂) ->
-          dnnrc_type tenv (DNNRCFor a v e1 e2) (Tlocal (Coll τ₂))
+          dnnrc_base_type tenv e1 (Tlocal (Coll τ₁)) ->
+          dnnrc_base_type ((v,(Tlocal τ₁))::tenv) e2 (Tlocal τ₂) ->
+          dnnrc_base_type tenv (DNNRCFor a v e1 e2) (Tlocal (Coll τ₂))
     | TDNNRCForDist {τ₁ τ₂} v tenv e1 e2 :
         forall (a:A),
-          dnnrc_type tenv e1 (Tdistr τ₁) ->
-          dnnrc_type ((v,(Tlocal τ₁))::tenv) e2 (Tlocal τ₂) ->
-          dnnrc_type tenv (DNNRCFor a v e1 e2) (Tdistr τ₂)
+          dnnrc_base_type tenv e1 (Tdistr τ₁) ->
+          dnnrc_base_type ((v,(Tlocal τ₁))::tenv) e2 (Tlocal τ₂) ->
+          dnnrc_base_type tenv (DNNRCFor a v e1 e2) (Tdistr τ₂)
     | TDNNRCIf {τout} tenv e1 e2 e3 :
         forall (a:A), 
-          dnnrc_type tenv e1 (Tlocal Bool) ->
-          dnnrc_type tenv e2 τout ->
-          dnnrc_type tenv e3 τout ->
-          dnnrc_type tenv (DNNRCIf a e1 e2 e3) τout
+          dnnrc_base_type tenv e1 (Tlocal Bool) ->
+          dnnrc_base_type tenv e2 τout ->
+          dnnrc_base_type tenv e3 τout ->
+          dnnrc_base_type tenv (DNNRCIf a e1 e2 e3) τout
     | TDNNRCEither {τout τl τr} tenv ed xl el xr er :
         forall (a:A), 
-          dnnrc_type tenv ed (Tlocal (Either τl τr)) ->
-          dnnrc_type ((xl,(Tlocal τl))::tenv) el τout ->
-          dnnrc_type ((xr,(Tlocal τr))::tenv) er τout ->
-          dnnrc_type tenv (DNNRCEither a ed xl el xr er) τout
+          dnnrc_base_type tenv ed (Tlocal (Either τl τr)) ->
+          dnnrc_base_type ((xl,(Tlocal τl))::tenv) el τout ->
+          dnnrc_base_type ((xr,(Tlocal τr))::tenv) er τout ->
+          dnnrc_base_type tenv (DNNRCEither a ed xl el xr er) τout
     | TDNNRCCollect {τ} tenv e :
         forall (a:A),
-          dnnrc_type tenv e (Tdistr τ) ->
-          dnnrc_type tenv (DNNRCCollect a e) (Tlocal (Coll τ))
+          dnnrc_base_type tenv e (Tdistr τ) ->
+          dnnrc_base_type tenv (DNNRCCollect a e) (Tlocal (Coll τ))
     | TDNNRCDispatch {τ} tenv e :
         forall (a:A),
-          dnnrc_type tenv e (Tlocal (Coll τ)) ->
-          dnnrc_type tenv (DNNRCDispatch a e) (Tdistr τ)
+          dnnrc_base_type tenv e (Tlocal (Coll τ)) ->
+          dnnrc_base_type tenv (DNNRCDispatch a e) (Tdistr τ)
     (* Note: algebra 'plugged' expression is only well typed within distributed
          NNNRC if it returns a collection *)
     | TDNNRCAlg {τout} tenv tbindings op nl :
         forall (a:A),
           Forall2 (fun n τ => fst n = fst τ
-                              /\ dnnrc_type tenv (snd n) (Tdistr (snd τ)))
+                              /\ dnnrc_base_type tenv (snd n) (Tdistr (snd τ)))
                   nl tbindings ->
           plug_typing op tbindings (Coll τout) -> 
-          dnnrc_type tenv (DNNRCAlg a op nl) (Tdistr τout)
+          dnnrc_base_type tenv (DNNRCAlg a op nl) (Tdistr τout)
     .
 
-    (* Print dnnrc_type_ind. We will need a special inductive principle because of the list of expressions in TDNRAlg *)
+    (* Print dnnrc_base_type_ind. We will need a special inductive principle because of the list of expressions in TDNRAlg *)
   End typ.
 
   (** Main lemma for the type correctness of DNNRC *)
@@ -186,11 +186,11 @@ Section TDNNRCBase.
       congruence.
   Qed.      
 
-  Theorem typed_dnnrc_yields_typed_data {A:Set} {plug_type:Set} {τc} {τ} `{tplug:TAlgPlug plug_type} (cenv env:dbindings) (tenv:tdbindings) (e:@dnnrc _ A plug_type) :
+  Theorem typed_dnnrc_base_yields_typed_data {A:Set} {plug_type:Set} {τc} {τ} `{tplug:TAlgPlug plug_type} (cenv env:dbindings) (tenv:tdbindings) (e:@dnnrc_base _ A plug_type) :
     dbindings_type cenv τc ->
     dbindings_type env tenv ->
-    dnnrc_type τc tenv e τ ->
-    (exists x, (dnnrc_eval brand_relation_brands cenv env e) = Some x /\ (ddata_type x τ)).
+    dnnrc_base_type τc tenv e τ ->
+    (exists x, (dnnrc_base_eval brand_relation_brands cenv env e) = Some x /\ (ddata_type x τ)).
   Proof.
     intro Hcenv; intros.
     revert env H.
@@ -218,9 +218,9 @@ Section TDNNRCBase.
       assumption.
     - exists (Dlocal (normalize_data brand_relation_brands c)).
       intros. split; [reflexivity|constructor; assumption].
-    - specialize (IHdnnrc_type1 env H0); specialize (IHdnnrc_type2 env H0).
-      elim IHdnnrc_type1; intros; clear IHdnnrc_type1;
-      elim IHdnnrc_type2; intros; clear IHdnnrc_type2.
+    - specialize (IHdnnrc_base_type1 env H0); specialize (IHdnnrc_base_type2 env H0).
+      elim IHdnnrc_base_type1; intros; clear IHdnnrc_base_type1;
+      elim IHdnnrc_base_type2; intros; clear IHdnnrc_base_type2.
       elim H1; clear H1; intros.
       elim H2; clear H2; intros.
       rewrite H1; rewrite H2.
@@ -233,8 +233,8 @@ Section TDNNRCBase.
       split.
       + rewrite H3; reflexivity.
       + constructor; assumption.
-    - specialize (IHdnnrc_type env H1).
-      elim IHdnnrc_type; intros; clear IHdnnrc_type.
+    - specialize (IHdnnrc_base_type env H1).
+      elim IHdnnrc_base_type; intros; clear IHdnnrc_base_type.
       elim H2; clear H2; intros.
       rewrite H2; clear H2.
       inversion H3; clear H3; intros; subst.
@@ -244,14 +244,14 @@ Section TDNNRCBase.
       split.
       + rewrite H2; reflexivity.
       + constructor; assumption.
-    - destruct (IHdnnrc_type1 _ H) as [?[re1 ?]].
-      destruct (IHdnnrc_type2 ((v,x)::env)) as [?[re2 ?]].
+    - destruct (IHdnnrc_base_type1 _ H) as [?[re1 ?]].
+      destruct (IHdnnrc_base_type2 ((v,x)::env)) as [?[re2 ?]].
       + apply Forall2_cons; intuition.
       + unfold var in *.
         rewrite re1, re2.
         eauto.
-    - specialize (IHdnnrc_type1 env H).
-      elim IHdnnrc_type1; intros; clear IHdnnrc_type1.
+    - specialize (IHdnnrc_base_type1 env H).
+      elim IHdnnrc_base_type1; intros; clear IHdnnrc_base_type1.
       elim H0; clear H0; intros.
       rewrite H0; clear H0; simpl.
       inversion H1; clear H1; subst.
@@ -272,13 +272,13 @@ Section TDNNRCBase.
         assert (exists x1, rmap
            (fun d1 : data =>
             olift checkLocal
-              (dnnrc_eval brand_relation_brands cenv ((v, Dlocal d1) :: env) e2))
+              (dnnrc_base_eval brand_relation_brands cenv ((v, Dlocal d1) :: env) e2))
            dl = Some x1 /\ (Dlocal (dcoll x1)) = x0).
         revert H1.
         elim (rmap
        (fun d1 : data =>
         olift checkLocal
-              (dnnrc_eval brand_relation_brands cenv ((v, Dlocal d1) :: env) e2)) dl); intros.
+              (dnnrc_base_eval brand_relation_brands cenv ((v, Dlocal d1) :: env) e2)) dl); intros.
         inversion H1; simpl in *. subst; clear H1.
         exists a1; split; reflexivity.
         congruence.
@@ -286,7 +286,7 @@ Section TDNNRCBase.
         elim H3; clear H3; intros.
         rewrite H3.
         rewrite <- H4 in *; clear H1 H3 H4; simpl.
-        specialize (IHdnnrc_type2 ((v,Dlocal a0)::env)).
+        specialize (IHdnnrc_base_type2 ((v,Dlocal a0)::env)).
         assert (dbindings_type ((v, Dlocal a0) :: env) ((v, Tlocal τ₁) :: tenv)).
         unfold dbindings_type.
         apply Forall2_cons; try assumption.
@@ -294,8 +294,8 @@ Section TDNNRCBase.
         assert (r = τ₁) by (apply rtype_fequal; assumption).
         rewrite H1 in *; clear H1 x.
         constructor. apply (H0 a0); left; reflexivity.
-        specialize (IHdnnrc_type2 H1); clear H1.
-        elim IHdnnrc_type2; clear IHdnnrc_type2; intros.
+        specialize (IHdnnrc_base_type2 H1); clear H1.
+        elim IHdnnrc_base_type2; clear IHdnnrc_base_type2; intros.
         elim H1; clear H1; intros.
         rewrite H1; simpl.
         inversion H3; clear H3; subst.
@@ -310,8 +310,8 @@ Section TDNNRCBase.
         assert (r0 = τ₂) by (apply rtype_fequal; assumption).
         subst.
         apply (H2 x2); assumption.
-    - specialize (IHdnnrc_type1 env H).
-      elim IHdnnrc_type1; intros; clear IHdnnrc_type1.
+    - specialize (IHdnnrc_base_type1 env H).
+      elim IHdnnrc_base_type1; intros; clear IHdnnrc_base_type1.
       elim H0; clear H0; intros.
       rewrite H0; clear H0; simpl.
       inversion H1; clear H1; subst.
@@ -331,13 +331,13 @@ Section TDNNRCBase.
         assert (exists x1, rmap
            (fun d1 : data =>
             olift checkLocal
-              (dnnrc_eval brand_relation_brands cenv ((v, Dlocal d1) :: env) e2))
+              (dnnrc_base_eval brand_relation_brands cenv ((v, Dlocal d1) :: env) e2))
            dl = Some x1 /\ (Ddistr x1) = x).
         revert H0.
         elim (rmap
                 (fun d1 : data =>
                    olift checkLocal
-                         (dnnrc_eval brand_relation_brands cenv ((v, Dlocal d1) :: env) e2)) dl); intros.
+                         (dnnrc_base_eval brand_relation_brands cenv ((v, Dlocal d1) :: env) e2)) dl); intros.
         inversion H0; simpl in *. subst; clear H0.
         exists a1; split; reflexivity.
         congruence.
@@ -345,15 +345,15 @@ Section TDNNRCBase.
         elim H2; clear H2; intros.
         subst.
         inversion H1; subst.
-        specialize (IHdnnrc_type2 ((v,Dlocal a0)::env)).
+        specialize (IHdnnrc_base_type2 ((v,Dlocal a0)::env)).
         assert (dbindings_type ((v, Dlocal a0) :: env) ((v, Tlocal τ₁) :: tenv)).
         unfold dbindings_type.
         apply Forall2_cons; try assumption.
         simpl; split; try reflexivity.
         constructor.
         apply (H3 a0); left; reflexivity.
-        specialize (IHdnnrc_type2 H4); clear H4.
-        elim IHdnnrc_type2; clear IHdnnrc_type2; intros.
+        specialize (IHdnnrc_base_type2 H4); clear H4.
+        elim IHdnnrc_base_type2; clear IHdnnrc_base_type2; intros.
         elim H4; clear H4; intros.
         rewrite H4; simpl.
         inversion H5; clear H5; subst.
@@ -363,7 +363,7 @@ Section TDNNRCBase.
         elim (rmap
        (fun d1 : data =>
         olift checkLocal
-              (dnnrc_eval brand_relation_brands cenv ((v, Dlocal d1) :: env) e2)) dl); intros.
+              (dnnrc_base_eval brand_relation_brands cenv ((v, Dlocal d1) :: env) e2)) dl); intros.
         inversion H0.
         subst.
         reflexivity.
@@ -373,10 +373,10 @@ Section TDNNRCBase.
         elim H5; clear H5; intros.
         subst; assumption.
         auto.
-    - specialize (IHdnnrc_type1 env H); specialize (IHdnnrc_type2 env H); specialize (IHdnnrc_type3 env H).
-      elim IHdnnrc_type1; intros; clear IHdnnrc_type1;
-      elim IHdnnrc_type2; intros; clear IHdnnrc_type2;
-      elim IHdnnrc_type3; intros; clear IHdnnrc_type3.
+    - specialize (IHdnnrc_base_type1 env H); specialize (IHdnnrc_base_type2 env H); specialize (IHdnnrc_base_type3 env H).
+      elim IHdnnrc_base_type1; intros; clear IHdnnrc_base_type1;
+      elim IHdnnrc_base_type2; intros; clear IHdnnrc_base_type2;
+      elim IHdnnrc_base_type3; intros; clear IHdnnrc_base_type3.
       elim H0; clear H0; intros.
       elim H1; clear H1; intros.
       elim H2; clear H2; intros.
@@ -389,21 +389,21 @@ Section TDNNRCBase.
         exists x0; split; [reflexivity|assumption].
       + rewrite H2.
         exists x1; split; [reflexivity|assumption].
-    - destruct (IHdnnrc_type1 _ H) as [dd [evald typd]].
+    - destruct (IHdnnrc_base_type1 _ H) as [dd [evald typd]].
       inversion typd; clear typd; subst.
       apply data_type_Either_inv in H2.
       rewrite evald.
       simpl.
       destruct H2 as [[ddl[? typd]]|[ddr[? typd]]]; subst.
-      + destruct (IHdnnrc_type2 ((xl,Dlocal ddl)::env));
+      + destruct (IHdnnrc_base_type2 ((xl,Dlocal ddl)::env));
         unfold dbindings_type in *; auto.
         apply Forall2_cons; auto; split; [auto|constructor;auto].
         exists x; auto.
-      + destruct (IHdnnrc_type3 ((xr,Dlocal ddr)::env));
+      + destruct (IHdnnrc_base_type3 ((xr,Dlocal ddr)::env));
         unfold dbindings_type in *; auto.
         apply Forall2_cons; auto; split; [auto|constructor;auto].
         exists x; auto.
-    - elim (IHdnnrc_type env H); intros.
+    - elim (IHdnnrc_base_type env H); intros.
       elim H1; clear H1; intros.
       rewrite H1; simpl.
       inversion H2; clear H2; subst.
@@ -412,7 +412,7 @@ Section TDNNRCBase.
       constructor.
       constructor.
       assumption.
-    - elim (IHdnnrc_type env H); intros.
+    - elim (IHdnnrc_base_type env H); intros.
       elim H1; clear H1; intros.
       rewrite H1; simpl.
       inversion H2; clear H2; subst; simpl.
