coq/tDNNRC/Typing/tDNNRCSub.v
@@ -31,85 +31,85 @@ Section tDNNRCSub.
   Section typ.
     Context (τconstants:tdbindings).
       
-    Inductive dnnrc_type_sub {A plug_type:Set}
+    Inductive dnnrc_base_type_sub {A plug_type:Set}
               {plug:AlgPlug plug_type} {tplug: TAlgPlug} :
-      tdbindings -> @dnnrc _ A plug_type -> drtype -> Prop :=
+      tdbindings -> @dnnrc_base _ A plug_type -> drtype -> Prop :=
     | TDNNRCGetConstant {τout} tenv s :
         forall (a:A),
           tdot τconstants s = Some τout ->
-          dnnrc_type_sub tenv (DNNRCGetConstant a s) τout
+          dnnrc_base_type_sub tenv (DNNRCGetConstant a s) τout
     | TDNNRCVar {τ} tenv v :
         forall (a:A),
           lookup equiv_dec tenv v = Some τ ->
-          dnnrc_type_sub tenv (DNNRCVar a v) τ
+          dnnrc_base_type_sub tenv (DNNRCVar a v) τ
     | TDNNRCConst {τ} tenv c :
         forall (a:A),
           data_type (normalize_data brand_relation_brands c) τ ->
-          dnnrc_type_sub tenv (DNNRCConst a c) (Tlocal τ)
+          dnnrc_base_type_sub tenv (DNNRCConst a c) (Tlocal τ)
     | TDNNRCBinop  {τ₁ τ₂ τ} tenv b e1 e2 :
         forall (a:A),
           binOp_type b τ₁ τ₂ τ ->
-          dnnrc_type_sub tenv e1 (Tlocal τ₁) ->
-          dnnrc_type_sub tenv e2 (Tlocal τ₂) ->
-          dnnrc_type_sub tenv (DNNRCBinop a b e1 e2) (Tlocal τ)
+          dnnrc_base_type_sub tenv e1 (Tlocal τ₁) ->
+          dnnrc_base_type_sub tenv e2 (Tlocal τ₂) ->
+          dnnrc_base_type_sub tenv (DNNRCBinop a b e1 e2) (Tlocal τ)
     | TDNNRCUnop {τ₁ τ} tenv u e1 :
         forall (a:A), 
           unaryOp_type u τ₁ τ ->
-          dnnrc_type_sub tenv e1 (Tlocal τ₁) ->
-          dnnrc_type_sub tenv (DNNRCUnop a u e1) (Tlocal τ)
+          dnnrc_base_type_sub tenv e1 (Tlocal τ₁) ->
+          dnnrc_base_type_sub tenv (DNNRCUnop a u e1) (Tlocal τ)
     | TDNNRCLet {τ₁ τ₂} v tenv e1 e2 :
         forall (a:A), 
-          dnnrc_type_sub tenv e1 τ₁ ->
-          dnnrc_type_sub ((v,τ₁)::tenv) e2 τ₂ ->
-          dnnrc_type_sub tenv (DNNRCLet a v e1 e2) τ₂
+          dnnrc_base_type_sub tenv e1 τ₁ ->
+          dnnrc_base_type_sub ((v,τ₁)::tenv) e2 τ₂ ->
+          dnnrc_base_type_sub tenv (DNNRCLet a v e1 e2) τ₂
     | TDNRCForLocal {τ₁ τ₂} v tenv e1 e2 :
         forall (a:A),
-          dnnrc_type_sub tenv e1 (Tlocal (Coll τ₁)) ->
-          dnnrc_type_sub ((v,(Tlocal τ₁))::tenv) e2 (Tlocal τ₂) ->
-          dnnrc_type_sub tenv (DNNRCFor a v e1 e2) (Tlocal (Coll τ₂))
+          dnnrc_base_type_sub tenv e1 (Tlocal (Coll τ₁)) ->
+          dnnrc_base_type_sub ((v,(Tlocal τ₁))::tenv) e2 (Tlocal τ₂) ->
+          dnnrc_base_type_sub tenv (DNNRCFor a v e1 e2) (Tlocal (Coll τ₂))
     | TDNRCForDist {τ₁ τ₂} v tenv e1 e2 :
         forall (a:A),
-          dnnrc_type_sub tenv e1 (Tdistr τ₁) ->
-          dnnrc_type_sub ((v,(Tlocal τ₁))::tenv) e2 (Tlocal τ₂) ->
-          dnnrc_type_sub tenv (DNNRCFor a v e1 e2) (Tdistr τ₂)                      
+          dnnrc_base_type_sub tenv e1 (Tdistr τ₁) ->
+          dnnrc_base_type_sub ((v,(Tlocal τ₁))::tenv) e2 (Tlocal τ₂) ->
+          dnnrc_base_type_sub tenv (DNNRCFor a v e1 e2) (Tdistr τ₂)                      
     | TDNRCIf {τ} tenv e1 e2 e3 :
         forall (a:A), 
-          dnnrc_type_sub tenv e1 (Tlocal Bool) ->
-          dnnrc_type_sub tenv e2 τ ->
-          dnnrc_type_sub tenv e3 τ ->
-          dnnrc_type_sub tenv (DNNRCIf a e1 e2 e3) τ
+          dnnrc_base_type_sub tenv e1 (Tlocal Bool) ->
+          dnnrc_base_type_sub tenv e2 τ ->
+          dnnrc_base_type_sub tenv e3 τ ->
+          dnnrc_base_type_sub tenv (DNNRCIf a e1 e2 e3) τ
     | TDNNRCEither {τ τl τr} tenv ed xl el xr er :
         forall (a:A), 
-          dnnrc_type_sub tenv ed (Tlocal (Either τl τr)) ->
-          dnnrc_type_sub ((xl,(Tlocal τl))::tenv) el τ ->
-          dnnrc_type_sub ((xr,(Tlocal τr))::tenv) er τ ->
-          dnnrc_type_sub tenv (DNNRCEither a ed xl el xr er) τ
+          dnnrc_base_type_sub tenv ed (Tlocal (Either τl τr)) ->
+          dnnrc_base_type_sub ((xl,(Tlocal τl))::tenv) el τ ->
+          dnnrc_base_type_sub ((xr,(Tlocal τr))::tenv) er τ ->
+          dnnrc_base_type_sub tenv (DNNRCEither a ed xl el xr er) τ
     | TDNNRCCollect {τ} tenv e :
         forall (a:A),
-          dnnrc_type_sub tenv e (Tdistr τ) ->
-          dnnrc_type_sub tenv (DNNRCCollect a e) (Tlocal (Coll τ))
+          dnnrc_base_type_sub tenv e (Tdistr τ) ->
+          dnnrc_base_type_sub tenv (DNNRCCollect a e) (Tlocal (Coll τ))
     | TDNNRCDispatch {τ} tenv e :
         forall (a:A),
-          dnnrc_type_sub tenv e (Tlocal (Coll τ)) ->
-          dnnrc_type_sub tenv (DNNRCDispatch a e) (Tdistr τ)
+          dnnrc_base_type_sub tenv e (Tlocal (Coll τ)) ->
+          dnnrc_base_type_sub tenv (DNNRCDispatch a e) (Tdistr τ)
     (* Note: algebra 'plugged' expression is only well typed within distributed
          NNNRC if it returns a collection *)
     | TDNNRCAlg {τout} tenv tbindings op nl :
         forall (a:A),
           Forall2 (fun n τ => fst n = fst τ
-                              /\ dnnrc_type_sub tenv (snd n) (Tdistr (snd τ)))
+                              /\ dnnrc_base_type_sub tenv (snd n) (Tdistr (snd τ)))
                   nl tbindings ->
           plug_typing op tbindings (Coll τout) -> 
-          dnnrc_type_sub tenv (DNNRCAlg a op nl) (Tdistr τout)
+          dnnrc_base_type_sub tenv (DNNRCAlg a op nl) (Tdistr τout)
     | TDNNRCSubsumption {τenv τout} τenv' τout' e:
         tdbindings_sub τenv' τenv ->
         drtype_sub τout τout' ->
-        dnnrc_type_sub τenv e τout ->
-        dnnrc_type_sub τenv' e τout'
+        dnnrc_base_type_sub τenv e τout ->
+        dnnrc_base_type_sub τenv' e τout'
     .
 
-    Global Instance dnnrc_type_sub_proper {A plug_type:Set} {plug:AlgPlug plug_type} {tplug: TAlgPlug} :
-      Proper (tdbindings_sub --> eq ==> drtype_sub ==> impl) (dnnrc_type_sub (A:=A)).
+    Global Instance dnnrc_base_type_sub_proper {A plug_type:Set} {plug:AlgPlug plug_type} {tplug: TAlgPlug} :
+      Proper (tdbindings_sub --> eq ==> drtype_sub ==> impl) (dnnrc_base_type_sub (A:=A)).
     Proof.
       unfold Proper, respectful, flip, impl; intros.
       subst.
@@ -133,11 +133,11 @@ Section tDNNRCSub.
 
   Section lift.
     
-    Lemma dnnrc_type_to_dnnrc_type_sub {A} (plug_type:Set) (plug:AlgPlug plug_type) {tplug:TAlgPlug} {τc} {τ} (tenv:tdbindings) (e:@dnnrc _ A plug_type) :
-      dnnrc_type τc tenv e τ ->
-      dnnrc_type_sub τc tenv e τ.
+    Lemma dnnrc_base_type_to_dnnrc_base_type_sub {A} (plug_type:Set) (plug:AlgPlug plug_type) {tplug:TAlgPlug} {τc} {τ} (tenv:tdbindings) (e:@dnnrc_base _ A plug_type) :
+      dnnrc_base_type τc tenv e τ ->
+      dnnrc_base_type_sub τc tenv e τ.
     Proof.
-      Hint Constructors dnnrc_type_sub.
+      Hint Constructors dnnrc_base_type_sub.
       revert tenv τ.
       induction e; simpl; intros tenv τ dt; invcs dt; eauto.
       - econstructor; try eassumption.
@@ -151,11 +151,11 @@ Section tDNNRCSub.
   End lift.
   
 (** Main lemma for the type correctness of DNNNRC *)
-  Theorem typed_dnnrc_yields_typed_data {A} {plug_type:Set} (plug:AlgPlug plug_type) {tplug:TAlgPlug} {τc} {τ} (cenv env:dbindings) (tenv:tdbindings) (e:@dnnrc _ A plug_type) :
+  Theorem typed_dnnrc_base_yields_typed_data {A} {plug_type:Set} (plug:AlgPlug plug_type) {tplug:TAlgPlug} {τc} {τ} (cenv env:dbindings) (tenv:tdbindings) (e:@dnnrc_base _ A plug_type) :
     dbindings_type cenv τc ->
     dbindings_type env tenv ->
-    dnnrc_type_sub τc tenv e τ ->
-    (exists x, (dnnrc_eval brand_relation_brands cenv env e) = Some x /\ (ddata_type x τ)).
+    dnnrc_base_type_sub τc tenv e τ ->
+    (exists x, (dnnrc_base_eval brand_relation_brands cenv env e) = Some x /\ (ddata_type x τ)).
   Proof.
     intro Hcenv; intros.
     revert env H.
@@ -183,9 +183,9 @@ Section tDNNRCSub.
       assumption.
     - exists (Dlocal (normalize_data brand_relation_brands c)).
       intros. split; [reflexivity|constructor; assumption].
-    - specialize (IHdnnrc_type_sub1 env H0); specialize (IHdnnrc_type_sub2 env H0).
-      elim IHdnnrc_type_sub1; intros; clear IHdnnrc_type_sub1;
-        elim IHdnnrc_type_sub2; intros; clear IHdnnrc_type_sub2.
+    - specialize (IHdnnrc_base_type_sub1 env H0); specialize (IHdnnrc_base_type_sub2 env H0).
+      elim IHdnnrc_base_type_sub1; intros; clear IHdnnrc_base_type_sub1;
+        elim IHdnnrc_base_type_sub2; intros; clear IHdnnrc_base_type_sub2.
       elim H1; clear H1; intros.
       elim H2; clear H2; intros.
       rewrite H1; rewrite H2.
@@ -198,8 +198,8 @@ Section tDNNRCSub.
       split.
       + rewrite H3; reflexivity.
       + constructor; assumption.
-    - specialize (IHdnnrc_type_sub env H1).
-      elim IHdnnrc_type_sub; intros; clear IHdnnrc_type_sub.
+    - specialize (IHdnnrc_base_type_sub env H1).
+      elim IHdnnrc_base_type_sub; intros; clear IHdnnrc_base_type_sub.
       elim H2; clear H2; intros.
       rewrite H2; clear H2.
       inversion H3; clear H3; intros; subst.
@@ -209,18 +209,18 @@ Section tDNNRCSub.
       split.
       + rewrite H2; reflexivity.
       + constructor; assumption.
-    - destruct (IHdnnrc_type_sub1 _ H) as [?[re1 ?]].
-      destruct (IHdnnrc_type_sub2 ((v,x)::env)) as [?[re2 ?]].
+    - destruct (IHdnnrc_base_type_sub1 _ H) as [?[re1 ?]].
+      destruct (IHdnnrc_base_type_sub2 ((v,x)::env)) as [?[re2 ?]].
       + apply Forall2_cons; intuition.
       + unfold var in *.
         rewrite re1.
-        assert ((@dnnrc_eval (@basic_model_runtime m) A plug_type
+        assert ((@dnnrc_base_eval (@basic_model_runtime m) A plug_type
              (@brand_relation_brands
                 (@brand_model_relation (@basic_model_foreign_type m)
                    (@basic_model_brand_model m))) cenv plug
              (@cons (prod string (@ddata (@foreign_runtime_data (@basic_model_runtime m))))
                 (@pair string (@ddata (@foreign_runtime_data (@basic_model_runtime m))) v x)
-                env) e2) = (@dnnrc_eval (@basic_model_runtime m) A plug_type
+                env) e2) = (@dnnrc_base_eval (@basic_model_runtime m) A plug_type
              (@brand_relation_brands
                 (@brand_model_relation (@basic_model_foreign_type m)
                    (@basic_model_brand_model m))) cenv plug
@@ -231,8 +231,8 @@ Section tDNNRCSub.
         rewrite H2 in re2; clear H2.
         rewrite re2.
         eauto.
-    - specialize (IHdnnrc_type_sub1 env H).
-      elim IHdnnrc_type_sub1; intros; clear IHdnnrc_type_sub1.
+    - specialize (IHdnnrc_base_type_sub1 env H).
+      elim IHdnnrc_base_type_sub1; intros; clear IHdnnrc_base_type_sub1.
       elim H0; clear H0; intros.
       rewrite H0; clear H0; simpl.
       inversion H1; clear H1; subst.
@@ -253,7 +253,7 @@ Section tDNNRCSub.
         assert (exists x1, rmap
            (fun d1 : data =>
             olift checkLocal
-              (dnnrc_eval brand_relation_brands cenv ((v, Dlocal d1) :: env) e2))
+              (dnnrc_base_eval brand_relation_brands cenv ((v, Dlocal d1) :: env) e2))
            dl = Some x1 /\ (Dlocal (dcoll x1)) = x0).
         revert H1.
         assert (@rmap (@data (@foreign_runtime_data (@basic_model_runtime m)))
@@ -262,7 +262,7 @@ Section tDNNRCSub.
                @olift (@ddata (@foreign_runtime_data (@basic_model_runtime m)))
                  (@data (@foreign_runtime_data (@basic_model_runtime m)))
                  (@checkLocal (@foreign_runtime_data (@basic_model_runtime m)))
-                 (@dnnrc_eval (@basic_model_runtime m) A plug_type
+                 (@dnnrc_base_eval (@basic_model_runtime m) A plug_type
                     (@brand_relation_brands
                        (@brand_model_relation (@basic_model_foreign_type m)
                           (@basic_model_brand_model m))) cenv plug
@@ -278,7 +278,7 @@ Section tDNNRCSub.
               @olift (@ddata (@foreign_runtime_data (@basic_model_runtime m)))
                 (@data (@foreign_runtime_data (@basic_model_runtime m)))
                 (@checkLocal (@foreign_runtime_data (@basic_model_runtime m)))
-                (@dnnrc_eval (@basic_model_runtime m) A plug_type
+                (@dnnrc_base_eval (@basic_model_runtime m) A plug_type
                    (@brand_relation_brands
                       (@brand_model_relation (@basic_model_foreign_type m)
                          (@basic_model_brand_model m))) cenv plug
@@ -291,7 +291,7 @@ Section tDNNRCSub.
         elim (rmap
                 (fun d1 : data =>
                    olift checkLocal
-                         (dnnrc_eval brand_relation_brands cenv ((v, Dlocal d1) :: env) e2)) dl); intros.
+                         (dnnrc_base_eval brand_relation_brands cenv ((v, Dlocal d1) :: env) e2)) dl); intros.
         inversion H1; simpl in *. subst; clear H1;
         exists a1; split; congruence.
         congruence.
@@ -303,7 +303,7 @@ Section tDNNRCSub.
              @olift (@ddata (@foreign_runtime_data (@basic_model_runtime m)))
                (@data (@foreign_runtime_data (@basic_model_runtime m)))
                (@checkLocal (@foreign_runtime_data (@basic_model_runtime m)))
-               (@dnnrc_eval (@basic_model_runtime m) A plug_type
+               (@dnnrc_base_eval (@basic_model_runtime m) A plug_type
                   (@brand_relation_brands
                      (@brand_model_relation (@basic_model_foreign_type m)
                         (@basic_model_brand_model m))) cenv plug
@@ -317,7 +317,7 @@ Section tDNNRCSub.
                        @olift (@ddata (@foreign_runtime_data (@basic_model_runtime m)))
                          (@data (@foreign_runtime_data (@basic_model_runtime m)))
                          (@checkLocal (@foreign_runtime_data (@basic_model_runtime m)))
-                         (@dnnrc_eval (@basic_model_runtime m) A plug_type
+                         (@dnnrc_base_eval (@basic_model_runtime m) A plug_type
                             (@brand_relation_brands
                                (@brand_model_relation (@basic_model_foreign_type m)
                                   (@basic_model_brand_model m))) cenv plug
@@ -331,7 +331,7 @@ Section tDNNRCSub.
         rewrite <- H5; clear H5.
         rewrite H3.
         rewrite <- H4 in *; clear H1 H3 H4; simpl.
-        specialize (IHdnnrc_type_sub2 ((v,Dlocal a0)::env)).
+        specialize (IHdnnrc_base_type_sub2 ((v,Dlocal a0)::env)).
         assert (dbindings_type ((v, Dlocal a0) :: env) ((v, Tlocal τ₁) :: tenv)).
         unfold dbindings_type.
         apply Forall2_cons; try assumption.
@@ -339,17 +339,17 @@ Section tDNNRCSub.
         assert (r = τ₁) by (apply rtype_fequal; assumption).
         rewrite H1 in *; clear H1 x.
         constructor. apply (H0 a0); left; reflexivity.
-        specialize (IHdnnrc_type_sub2 H1); clear H1.
-        elim IHdnnrc_type_sub2; clear IHdnnrc_type_sub2; intros.
+        specialize (IHdnnrc_base_type_sub2 H1); clear H1.
+        elim IHdnnrc_base_type_sub2; clear IHdnnrc_base_type_sub2; intros.
         elim H1; clear H1; intros.
-        assert ((@dnnrc_eval (@basic_model_runtime m) A plug_type
+        assert ((@dnnrc_base_eval (@basic_model_runtime m) A plug_type
             (@brand_relation_brands
                (@brand_model_relation (@basic_model_foreign_type m)
                   (@basic_model_brand_model m))) cenv plug
             (@cons (prod string (@ddata (@foreign_runtime_data (@basic_model_runtime m))))
                (@pair string (@ddata (@foreign_runtime_data (@basic_model_runtime m))) v
                   (@Dlocal (@foreign_runtime_data (@basic_model_runtime m)) a0)) env) e2) =
-               (@dnnrc_eval (@basic_model_runtime m) A plug_type
+               (@dnnrc_base_eval (@basic_model_runtime m) A plug_type
                     (@brand_relation_brands
                        (@brand_model_relation (@basic_model_foreign_type m)
                           (@basic_model_brand_model m))) cenv plug
@@ -375,10 +375,10 @@ Section tDNNRCSub.
         subst.
         apply (H2 x2); assumption.
     - admit.
-    - specialize (IHdnnrc_type_sub1 env H); specialize (IHdnnrc_type_sub2 env H); specialize (IHdnnrc_type_sub3 env H).
-      elim IHdnnrc_type_sub1; intros; clear IHdnnrc_type_sub1;
-      elim IHdnnrc_type_sub2; intros; clear IHdnnrc_type_sub2;
-      elim IHdnnrc_type_sub3; intros; clear IHdnnrc_type_sub3.
+    - specialize (IHdnnrc_base_type_sub1 env H); specialize (IHdnnrc_base_type_sub2 env H); specialize (IHdnnrc_base_type_sub3 env H).
+      elim IHdnnrc_base_type_sub1; intros; clear IHdnnrc_base_type_sub1;
+      elim IHdnnrc_base_type_sub2; intros; clear IHdnnrc_base_type_sub2;
+      elim IHdnnrc_base_type_sub3; intros; clear IHdnnrc_base_type_sub3.
       elim H0; clear H0; intros.
       elim H1; clear H1; intros.
       elim H2; clear H2; intros.
@@ -391,21 +391,21 @@ Section tDNNRCSub.
         exists x0; split; [reflexivity|assumption].
       + rewrite H2.
         exists x1; split; [reflexivity|assumption].
-    - destruct (IHdnnrc_type_sub1 _ H) as [dd [evald typd]].
+    - destruct (IHdnnrc_base_type_sub1 _ H) as [dd [evald typd]].
       inversion typd; clear typd; subst.
       apply data_type_Either_inv in H2.
       rewrite evald.
       simpl.
       destruct H2 as [[ddl[? typd]]|[ddr[? typd]]]; subst.
-      + destruct (IHdnnrc_type_sub2 ((xl,Dlocal ddl)::env));
+      + destruct (IHdnnrc_base_type_sub2 ((xl,Dlocal ddl)::env));
         unfold dbindings_type in *; auto.
         apply Forall2_cons; auto; split; [auto|constructor;auto].
         exists x; auto.
-      + destruct (IHdnnrc_type_sub3 ((xr,Dlocal ddr)::env));
+      + destruct (IHdnnrc_base_type_sub3 ((xr,Dlocal ddr)::env));
         unfold dbindings_type in *; auto.
         apply Forall2_cons; auto; split; [auto|constructor;auto].
         exists x; auto.
-    - elim (IHdnnrc_type_sub env H); intros.
+    - elim (IHdnnrc_base_type_sub env H); intros.
       elim H1; clear H1; intros.
       rewrite H1; simpl.
       inversion H2; clear H2; subst.
@@ -414,7 +414,7 @@ Section tDNNRCSub.
       constructor.
       constructor.
       assumption.
-    - elim (IHdnnrc_type_sub env H); intros.
+    - elim (IHdnnrc_base_type_sub env H); intros.
       elim H1; clear H1; intros.
       rewrite H1; simpl.
       inversion H2; clear H2; subst; simpl.
@@ -427,7 +427,7 @@ Section tDNNRCSub.
     - admit.
       (* We will need a special inductive principle because of the list of expressions in TDNRAlg *)
     - rewrite H in H2.
-      destruct (IHdnnrc_type_sub _ H2) as [dd [dd_eval dd_typ]].
+      destruct (IHdnnrc_base_type_sub _ H2) as [dd [dd_eval dd_typ]].
       rewrite H0 in dd_typ.
       eauto.
   Admitted.
