coq/Compiler/Model/CompilerModel.v
@@ -34,7 +34,6 @@ Require Import cNNRC.
 Require Import cNRAEnv.
 Require Import NRAEnv.
 Require Import DNNRC.
-Require Import Dataframe.
 Require Import tDNNRC.
 
 Module Type CompilerModel.
@@ -51,7 +50,7 @@ Module Type CompilerModel.
   Axiom compiler_model_foreign_to_cloudant : foreign_to_cloudant.
   Axiom compiler_model_nraenv_optimizer_logger : optimizer_logger string nraenv.
   Axiom compiler_model_nnrc_optimizer_logger : optimizer_logger string nnrc.
-  Axiom compiler_model_dnnrc_optimizer_logger : forall {br:brand_relation}, optimizer_logger string (dnnrc_dataframe_typed).
+  Axiom compiler_model_dnnrc_optimizer_logger : forall {br:brand_relation}, optimizer_logger string (dnnrc_typed).
   Axiom compiler_model_foreign_data_typing : foreign_data_typing.
 End CompilerModel.
 
@@ -84,7 +83,7 @@ Module CompilerModelRuntime(model:CompilerModel) <: CompilerRuntime.
     :=  model.compiler_model_nraenv_optimizer_logger.
   Definition compiler_nnrc_optimizer_logger : optimizer_logger string nnrc
     :=  model.compiler_model_nnrc_optimizer_logger.
-  Definition compiler_dnnrc_optimizer_logger {br:brand_relation}: optimizer_logger string  (dnnrc_dataframe_typed)
+  Definition compiler_dnnrc_optimizer_logger {br:brand_relation}: optimizer_logger string  (dnnrc_typed)
     :=  model.compiler_model_dnnrc_optimizer_logger.
   Definition compiler_foreign_data_typing : foreign_data_typing
     := model.compiler_model_foreign_data_typing.
