coq/Compiler/Model/CompilerRuntime.v
@@ -34,7 +34,6 @@ Require Import cNRAEnv.
 Require Import NRAEnv.
 Require Import DNNRC.
 Require Import tDNNRC.
-Require Import Dataframe.
 
 Module Type CompilerRuntime.
   Axiom compiler_foreign_type : foreign_type.
@@ -51,7 +50,7 @@ Module Type CompilerRuntime.
   Axiom compiler_foreign_to_cloudant : foreign_to_cloudant.
   Axiom compiler_nraenv_optimizer_logger : optimizer_logger string nraenv.
   Axiom compiler_nnrc_optimizer_logger : optimizer_logger string nnrc.
-  Axiom compiler_dnnrc_optimizer_logger : forall {br:brand_relation}, optimizer_logger string (dnnrc_dataframe_typed).
+  Axiom compiler_dnnrc_optimizer_logger : forall {br:brand_relation}, optimizer_logger string (dnnrc_typed).
   Axiom compiler_foreign_data_typing : foreign_data_typing.
 End CompilerRuntime.
 
