coq/Compiler/Model/TrivialModel.v
@@ -359,8 +359,8 @@ Existing Instance silent_optimizer_logger.
       := silent_optimizer_logger string nraenv.
     Definition compiler_nnrc_optimizer_logger : optimizer_logger string nnrc
       := silent_optimizer_logger string nnrc.
-    Definition compiler_dnnrc_optimizer_logger {br:brand_relation}: optimizer_logger string (@dnnrc _ (type_annotation unit) dataframe)
-      := silent_optimizer_logger string (@dnnrc _ (type_annotation unit) dataframe).
+    Definition compiler_dnnrc_optimizer_logger {br:brand_relation}: optimizer_logger string (@dnnrc_base _ (type_annotation unit) dataframe)
+      := silent_optimizer_logger string (@dnnrc_base _ (type_annotation unit) dataframe).
     Definition compiler_foreign_data_typing : foreign_data_typing
       := trivial_foreign_data_typing.
     
@@ -400,8 +400,8 @@ Existing Instance silent_optimizer_logger.
       := silent_optimizer_logger string nraenv.
     Definition compiler_model_nnrc_optimizer_logger : optimizer_logger string nnrc
       := silent_optimizer_logger string nnrc.
-    Definition compiler_model_dnnrc_optimizer_logger {br:brand_relation}: optimizer_logger string (@dnnrc _ (type_annotation unit) dataframe)
-      := silent_optimizer_logger string (@dnnrc _ (type_annotation unit) dataframe).
+    Definition compiler_model_dnnrc_optimizer_logger {br:brand_relation}: optimizer_logger string (@dnnrc_base _ (type_annotation unit) dataframe)
+      := silent_optimizer_logger string (@dnnrc_base _ (type_annotation unit) dataframe).
     Definition compiler_model_foreign_data_typing : foreign_data_typing
       := trivial_foreign_data_typing.
   End TrivialModel.
