coq/Translation/DNNRCtotDNNRC.v
@@ -25,8 +25,8 @@ Section DNNRCtotDNNRC.
     Context {bm:brand_model}.
     Context {ftyping: foreign_typing}.
 
-    Definition dnnrc_to_dnnrc_typed_top (tdenv: tdbindings) (q:dnnrc_dataframe) : option dnnrc_dataframe_typed :=
-      infer_dnnrc_type tdenv nil q.
+    Definition dnnrc_to_dnnrc_typed_top (tdenv: tdbindings) (q:dnnrc) : option dnnrc_typed :=
+      infer_dnnrc_base_type tdenv nil q.
 
   End Top.
   
