coq/Translation/NNRCMRtoDNNRC.v
@@ -44,11 +44,11 @@ Section NNRCMRtoDNNRC.
   (* Generates the DNNRC code corresponding to "(fun x => e1) e2" that is:
        let x = e2 in e1
    *)
-  Definition gen_apply_fun (annot:A) (f: var * nnrc) (e2: @dnnrc _ A plug_type) : (@dnnrc _ A plug_type) :=
+  Definition gen_apply_fun (annot:A) (f: var * nnrc) (e2: @dnnrc_base _ A plug_type) : (@dnnrc_base _ A plug_type) :=
     let (x, e1) := f in
     DNNRCLet annot
             x e2
-            (nnrc_to_dnnrc annot nil ((x, Vlocal)::nil) e1).
+            (nnrc_to_dnnrc_base annot nil ((x, Vlocal)::nil) e1).
 
   (* Generates the DNNRC code corresponding to "(fun (x1, ..., xn) => e) (e1, ..., en)" that is:
        let x1 = e1 in
@@ -56,7 +56,7 @@ Section NNRCMRtoDNNRC.
        let xn = en in
        e
    *)
-  Fixpoint gen_apply_fun_n (annot:A) (f: list var * nnrc)  (eff: list (var * dlocalization)) : option (@dnnrc _ A plug_type) :=
+  Fixpoint gen_apply_fun_n (annot:A) (f: list var * nnrc)  (eff: list (var * dlocalization)) : option (@dnnrc_base _ A plug_type) :=
     let (form, e) := f in
     match zip form eff with
     | Some l =>
@@ -74,62 +74,62 @@ Section NNRCMRtoDNNRC.
               DNNRCLet annot
                       x (DNNRCVar annot y)
                       k)
-           (nnrc_to_dnnrc annot form_loc nil e)
+           (nnrc_to_dnnrc_base annot form_loc nil e)
            l)
     | None => None
     end.
 
 
-  Definition dnnrc_distr_of_mr_map (annot:A) (input: var) (mr_map: map_fun) : (@dnnrc _ A plug_type) :=
+  Definition dnnrc_base_distr_of_mr_map (annot:A) (input: var) (mr_map: map_fun) : (@dnnrc_base _ A plug_type) :=
     match mr_map with
     | MapDist (x, n) =>
-      DNNRCFor annot x (DNNRCVar annot input) (nnrc_to_dnnrc annot nil ((x, Vlocal)::nil) n)
+      DNNRCFor annot x (DNNRCVar annot input) (nnrc_to_dnnrc_base annot nil ((x, Vlocal)::nil) n)
     | MapDistFlatten (x, n) =>
       let res_map :=
-          DNNRCFor annot x (DNNRCVar annot input) (nnrc_to_dnnrc annot nil ((x, Vlocal)::nil) n)
+          DNNRCFor annot x (DNNRCVar annot input) (nnrc_to_dnnrc_base annot nil ((x, Vlocal)::nil) n)
       in
       DNNRCUnop annot AFlatten res_map
     | MapScalar (x, n) =>
       let distr_input := DNNRCDispatch annot (DNNRCVar annot input) in
-      DNNRCFor annot x distr_input (nnrc_to_dnnrc annot nil ((x, Vlocal)::nil) n)
+      DNNRCFor annot x distr_input (nnrc_to_dnnrc_base annot nil ((x, Vlocal)::nil) n)
     end.
 
-  Definition dnnrc_local_of_mr_map (annot:A) (input: var) (mr_map: map_fun) : (@dnnrc _ A plug_type) :=
+  Definition dnnrc_base_local_of_mr_map (annot:A) (input: var) (mr_map: map_fun) : (@dnnrc_base _ A plug_type) :=
     match mr_map with
     | MapDist (x, n) =>
-      let res_map := DNNRCFor annot x (DNNRCVar annot input) (nnrc_to_dnnrc annot nil ((x, Vlocal)::nil) n) in
+      let res_map := DNNRCFor annot x (DNNRCVar annot input) (nnrc_to_dnnrc_base annot nil ((x, Vlocal)::nil) n) in
       DNNRCCollect annot res_map
     | MapDistFlatten (x, n) =>
-      let res_map := DNNRCFor annot x (DNNRCVar annot input) (nnrc_to_dnnrc annot nil ((x, Vlocal)::nil) n) in
+      let res_map := DNNRCFor annot x (DNNRCVar annot input) (nnrc_to_dnnrc_base annot nil ((x, Vlocal)::nil) n) in
       DNNRCCollect annot (DNNRCUnop annot AFlatten res_map)
     | MapScalar (x, n) =>
-      DNNRCFor annot x (DNNRCVar annot input) (nnrc_to_dnnrc annot nil ((x, Vlocal)::nil) n)
+      DNNRCFor annot x (DNNRCVar annot input) (nnrc_to_dnnrc_base annot nil ((x, Vlocal)::nil) n)
     end.
 
-  Definition dnnrc_of_mr (annot:A) (m:mr) : option (@dnnrc _ A plug_type) :=
+  Definition dnnrc_base_of_mr (annot:A) (m:mr) : option (@dnnrc_base _ A plug_type) :=
     match (m.(mr_map), m.(mr_reduce)) with
     | (MapScalar (x, NNRCUnop AColl n), RedSingleton) =>
       Some (gen_apply_fun annot (x, n) (DNNRCVar annot m.(mr_input)))
     | (_, RedSingleton) =>
       None
     | (map, RedId) =>
-      Some (dnnrc_distr_of_mr_map annot (mr_input m) map)
+      Some (dnnrc_base_distr_of_mr_map annot (mr_input m) map)
     | (map, RedCollect red_fun) =>
-      let map_expr := dnnrc_local_of_mr_map annot (mr_input m) map in
+      let map_expr := dnnrc_base_local_of_mr_map annot (mr_input m) map in
       Some (gen_apply_fun annot red_fun map_expr)
     | (map, RedOp op) =>
       match op with
       | RedOpForeign frop =>
-        let map_expr := dnnrc_distr_of_mr_map annot (mr_input m) map in
+        let map_expr := dnnrc_base_distr_of_mr_map annot (mr_input m) map in
         lift (fun op => DNNRCUnop annot op map_expr) (foreign_to_reduce_op_to_unary_op op)
       end
     end.
 
-  Fixpoint dnnrc_of_mr_chain (annot: A) (outputs: list var) (l: list mr) (k: @dnnrc _ A plug_type) : option (@dnnrc _ A plug_type) :=
+  Fixpoint dnnrc_base_of_mr_chain (annot: A) (outputs: list var) (l: list mr) (k: @dnnrc_base _ A plug_type) : option (@dnnrc_base _ A plug_type) :=
     match l with
     | nil => Some k
     | mr :: l =>
-      match (dnnrc_of_mr annot mr, dnnrc_of_mr_chain annot (mr_output mr :: outputs) l k) with
+      match (dnnrc_base_of_mr annot mr, dnnrc_base_of_mr_chain annot (mr_output mr :: outputs) l k) with
       | (Some n, Some k) =>
         Some (DNNRCLet annot
                       (mr_output mr)
@@ -141,12 +141,12 @@ Section NNRCMRtoDNNRC.
       end
     end.
 
-  Definition dnnrc_of_nnrcmr_top (annot: A) (l: nnrcmr) : option (@dnnrc _ A plug_type) :=
+  Definition dnnrc_base_of_nnrcmr_top (annot: A) (l: nnrcmr) : option (@dnnrc_base _ A plug_type) :=
     let constants := map fst (mr_inputs_loc l) in
     let (last_fun, last_args) :=  mr_last l in
     let k := gen_apply_fun_n annot last_fun last_args in
-    lift (dnnrc_subst_var_to_const constants)
-         (olift (dnnrc_of_mr_chain annot nil (mr_chain l)) k).
+    lift (dnnrc_base_subst_var_to_const constants)
+         (olift (dnnrc_base_of_mr_chain annot nil (mr_chain l)) k).
 
 End NNRCMRtoDNNRC.
 
